\begin{exercise}
	Evaluate the line integral, where $C$ is the given curve.
	\begin{equation*}
	\int_C xy \ ds, \quad C: x=t^2, \ y=2t, \ 0 \leq t \leq 1
	\end{equation*}
\end{exercise}
\begin{solution}
	The equation for the line integral of a curve $C$ is
	\begin{equation*}
	\int_C f\left(x,y\right) \ ds = \int_a^b f\left(x(t),y(t)\right)\sqrt{\left(\frac{dx}{dt}\right)^2+\left(\frac{dy}{dt}\right)^2}\ dt.
	\end{equation*}
	We thus begin by calculating the first partial derivatives with respect to $t$.
	\begin{align*}
	\frac{dx}{dt} &= \frac{d}{dt}\left(x(t)\right) \\
	&= \frac{d}{dt}\left(t^2\right)\\
	&= 2t
	\end{align*}
	\begin{align*}
	\frac{dy}{dt} &= \frac{d}{dt}\left(y(t)\right) \\
	&= \frac{d}{dt}\left(2t\right)\\
	&= 2
	\end{align*}
	We now plug in these values into the line integral equation, integrate, and simplify.
	\begin{align*}
	\int_C f\left(x,y\right) &= \int_a^b f\left(x(t),y(t)\right) \sqrt{ \left(\frac{dx}{dt}\right)^2 + \left(\frac{dy}{dt}\right)^2}\ dt \\
	&= \int_0^1 \left(t^2\right)\left(2t\right)\sqrt{\left(2t\right)^2+\left(2\right)^2}\ dt \\
	&= 2 \int_0^1 t^3 \sqrt{ 4t^2 + 4 }\ dt \\
	&= 4 \int_0^1 t^3 \sqrt{ t^2 + 1 }\ dt \\
	\intertext{Let $u = t^2 + 1$. Then $du = 2t\ dt$ and $t^2 = u - 1$.} \\
	&= 2 \int_1^2 \left( u - 1 \right)\left(\sqrt{u}\right)\ du \\
	&= 2 \left[ \int_1^2 u^{\frac{3}{2}}\ du - \int_1^2 u^{\frac{1}{2}}\ du \right] \\
	&= 2 \cdot \left( \left[ \frac{2}{5} u^{\frac{5}{2}} \right]_1^2 - \left[ \frac{2}{3} u^{\frac{3}{2}} \right]_1^2 \right) \\
	&= 2 \left( \left( \frac{2}{5} \left(2\right)^{\frac{5}{2}} - \frac{2}{5} \left(1\right)^{\frac{5}{2}} \right) - \left( \frac{2}{3} \left(2\right)^{\frac{3}{2}} - \frac{2}{3} \left(1\right)^{\frac{3}{2}} \right) \right) \\
	&= 4 \left[ \frac{1}{5} \left( 4\sqrt{2} - 1 \right) - \frac{1}{3} \left( 2\sqrt{2} - 1 \right) \right] \\
	&= \frac{4}{5}\left(4\sqrt{2} - 1\right) - \frac{4}{3}\left(2\sqrt{2} - 1\right) \\
	&= \frac{16\sqrt{2}}{5} - \frac{4}{5} - \frac{8\sqrt{2}}{3} + \frac{4}{3} \\
	&= \frac{48\sqrt{2}}{15} - \frac{12}{15} - \frac{40\sqrt{2}}{15} + \frac{20}{15} \\
	&= \frac{8+8\sqrt{2}}{15}
	\end{align*}
\end{solution}
